Finished CRC32 calculation.

code/c/Yazi_CRC32_Table_Codegen.c
@@ -1,12 +1,12 @@
 #include <stdio.h>
 #include <stdint.h>
-#include "Yazi_CRC32Table.h"
+#include "Yazi_CRC32_Table.h"
 
 int main(int argc, const char **argv) {
   uint32_t table[4][256];
   gen_crc32_table(table[0], table[1], table[2], table[3]);
 
-  printf("uint32_t crc32_table[4][256] = {\n");
+  printf("static uint32_t crc32_table[4][256] = {\n");
   
   for (int i = 0; i < 4; i++) {
     if (i == 0) {
@@ -26,7 +26,11 @@ int main(int argc, const char **argv) {
     }
   }
   
-  printf("\n};\n");
+  printf(
+    "\n};\n\n"
+    "unsigned long crc32(unsigned int crc, const unsigned char *buf, unsigned int len) {\n"
+    "  return Yazi_CRC32_crc32_impl((uint32_t *)crc32_table, crc, len, (uint8_t *) buf);\n"
+    "}\n");
   
   return 0;
 }
