code/Yazi.CRC32.fst
@@ -10,6 +10,67 @@ open FStar.Mul
 open FStar.Seq
 open LowStar.BufferOps
 open Spec.CRC32
+
+private unfold let do_pre_cond
+  (h: HS.mem)
+  (tg: table_group)
+  (p: crc32_current_state)
+  (d: crc32_init_state)
+  (i: nat)
+  (size: nat{size > 0}) =
+  let slen' = U32.v p.slen in
+  B.live h tg /\
+  B.live h p.stream /\
+  B.live h d.base /\  
+  B.disjoint p.stream tg /\
+  B.disjoint d.base tg /\
+
+  i + size <= d.blen /\
+  B.length p.stream == slen' /\
+  slen' >= size /\
+  slen' % size == 0 /\
+  slen' == d.blen - i /\
+  
+  Seq.length p.consumed == Ghost.reveal p.clen /\
+  B.length d.base == d.blen /\
+  Seq.length d.data == d.dlen /\
+
+  (let base' = B.as_seq h d.base in
+  let pending = Seq.slice base' i d.blen in
+  let consumed = Seq.slice base' 0 i in
+  Seq.equal (B.as_seq h p.stream) pending /\
+  Seq.equal (d.data @| consumed) p.consumed) /\
+  
+  crc32_matched p.clen p.consumed p.crc false /\
+  table_group_correct_pre h tg
+
+private unfold let do_post_cond
+  (h0 h1: HS.mem)
+  (tg: table_group)
+  (p: crc32_current_state)
+  (d: crc32_init_state)
+  (res: (U32.t & (B.buffer U8.t) & Ghost.erased (Seq.seq U8.t)))
+  (i: nat)
+  (size: nat{size > 0})
+  (next_size: option nat) =
+  let i' = match next_size with
+    | None -> i + size
+    | Some ns -> if ns > 0 then d.blen % ns else d.blen
+  in
+  let base' = B.as_seq h1 d.base in
+  let (crc', buf', data') = res in
+  B.(modifies loc_none h0 h1) /\
+  
+  B.length d.base == d.blen /\
+  Seq.length d.data == d.dlen /\
+  
+  B.live h1 buf' /\ B.disjoint buf' tg /\ B.length buf' == d.blen - i' /\
+
+  B.length buf' == d.blen - i' /\
+  Seq.equal (B.as_seq h1 buf') (Seq.slice base' i' d.blen) /\
+  Seq.equal data' (d.data @| (Seq.slice base' 0 i')) /\
+  
+  crc32_matched (d.dlen + i') data' crc' false
     
 #set-options "--z3rlimit 120 --z3seed 1 --fuel 16 --ifuel 16"
 let rec cast_zero_prefix (#n: nat) (v: UInt.uint_t n) (m: nat{m >= n}): Lemma
@@ -51,9 +112,7 @@ private unfold let u8_padding
   (b: U8.t)
   (n: nat{n > 0}):
   Tot (BV.bv_t (32 + 8 * n)) =
-  (BV.zero_vec #24) @|
-  (UInt.to_vec (U8.v b)) @|
-  (BV.zero_vec #(8 * n))
+  (BV.zero_vec #24) @| (UInt.to_vec (U8.v b)) @| BV.zero_vec #(8 * n)
 
 #set-options "--z3rlimit 120 --z3seed 13 --fuel 0 --ifuel 0"
 let do1_logxor
@@ -92,7 +151,7 @@ let do1_logxor
     assert(Seq.equal (zero_vec_l 24 (UInt.to_vec (U8.v b))) vb32)
   
 #set-options "--z3rlimit 200 --ifuel 128 --fuel 128 --z3seed 1"
-private let logand_256 (r: U32.t): Lemma
+let logand_256 (r: U32.t): Lemma
   (ensures forall (i: nat{i < 32}).
     (i < 32 - 8 ==> UInt.nth (U32.v (U32.logand r 0xFFul)) i == false) /\
     (i >= 32 - 8 ==> UInt.nth (U32.v (U32.logand r 0xFFul)) i == UInt.nth (U32.v r) i)) =
@@ -106,7 +165,7 @@ private let logand_256 (r: U32.t): Lemma
     (i >= 32 - 8 ==> UInt.nth (UInt.logand (v r) (v 0xFFul)) i == UInt.nth (U32.v r) i))
 
 #set-options "--z3seed 1 --fuel 0 --ifuel 0"
-private let do1_shift_right_logxor (r: U32.t) (t: U32.t): Lemma
+let do1_shift_right_logxor (r: U32.t) (t: U32.t): Lemma
   (requires poly_mod_correct 8 (U32.logand r 0xFFul) t)
   (ensures
      UInt.to_vec (U32.v (U32.logxor (U32.shift_right r 8ul) t)) ==
@@ -134,84 +193,66 @@ private let do1_shift_right_logxor (r: U32.t) (t: U32.t): Lemma
     ((zero_vec_r 8 vr') +@ (zero_vec_l 8 vi))
     (zero_vec_l 8 (UInt.to_vec (U32.v r))))
 
-#set-options "--z3rlimit 200 --z3seed 1 --fuel 1 --ifuel 1"
-inline_for_extraction
-private let do1
-  (m: Ghost.erased nat)
-  (data: Ghost.erased (Seq.seq U8.t){Seq.length data == Ghost.reveal m})
-  (t8: Spec.table_buf)
-  (crc: U32.t)
-  (b: U8.t):
-  ST.Stack (U32.t & (Ghost.erased (Seq.seq U8.t)))
-  (requires fun h -> table_correct 8 h t8 /\ crc32_matched m data crc false)
-  (ensures fun h0 res h1 ->
-    let crc' = fst res in
-    let data' = Ghost.reveal (snd res) in
-    B.modifies B.loc_none h0 h1 /\
-    data' == data @| (Seq.create 1 b) /\
-    crc32_matched (m + 1) data' crc' false) =
+#set-options "--z3rlimit 400 --z3seed 1 --fuel 1 --ifuel 1"
+inline_for_extraction let do1
+  (tg: table_group)
+  (p: crc32_current_state)
+  (d: Ghost.erased crc32_init_state)
+  (i: Ghost.erased nat):
+  ST.Stack (U32.t & (B.buffer U8.t) & Ghost.erased (Seq.seq U8.t))
+  (requires fun h -> do_pre_cond h tg p d i 1)
+  (ensures fun h0 res h1 -> do_post_cond h0 h1 tg p d res i 1 None) =
+  let b = p.stream.(0ul) in
   let b' = Cast.uint8_to_uint32 b in
   let open U32 in
-  let r = crc ^^ b' in
-  UInt.logand_le (v r) (v 0xFFul);
-  let tv = t8.(r &^ 0xFFul) in
+  let r = p.crc ^^ b' in
   let r' = r >>^ 8ul in
-  let p = r' ^^ tv in
-  let buf: Ghost.erased (BV.bv_t (if Ghost.reveal m = 0 then 0 else 32 + 8 * m)) =
-    Ghost.hide (crc32_data_to_bits m data)
+  UInt.logand_le (v r) (v 0xFFul);
+  
+  let (t8, _, _, _) = unfold_table_group tg in
+  let tv = t8.(r &^ 0xFFul) in
+
+  let crc' = r' ^^ tv in
+  let buf: Ghost.erased (BV.bv_t (if Ghost.reveal p.clen = 0 then 0 else 32 + 8 * p.clen)) =
+    Ghost.hide (crc32_data_to_bits p.clen p.consumed)
   in
-  do1_logxor m data crc b;
+  do1_logxor p.clen p.consumed p.crc b;
   do1_shift_right_logxor r tv;
 
-  if Ghost.reveal m > 0 then begin
-    poly_mod_zero_prefix (buf +@ (u8_padding b m)) 8;
-    crc32_data_to_bits_append m 1 data (Seq.create 1 b)
+  if Ghost.reveal p.clen > 0 then begin
+    poly_mod_zero_prefix (buf +@ (u8_padding b p.clen)) 8;
+    crc32_data_to_bits_append p.clen 1 p.consumed (Seq.create 1 b)
   end else
     assert(Seq.equal (zero_vec_l 8 (UInt.to_vec (v r))) (crc32_append_8bit buf b));
-    
-  (p, Ghost.hide (data @| (Seq.create 1 b)))
+
+  (crc', B.sub p.stream 1ul (p.slen -^ 1ul), Ghost.hide (Seq.snoc p.consumed b))
 
 #set-options "--z3rlimit 200 --ifuel 0 --fuel 0 --z3seed 7"
-inline_for_extraction
-private let rec do1_remain
-  (m: Ghost.erased nat)
-  (prev: Ghost.erased (Seq.seq U8.t){Seq.length prev == Ghost.reveal m})
-  (m': Ghost.erased nat)
-  (data: Ghost.erased (Seq.seq U8.t){Seq.length data == Ghost.reveal m'})
-  (t8: Spec.table_buf)
-  (l: U32.t{(U32.v l) % 4 > 0})
-  (r: U32.t{U32.v r < (U32.v l) % 4})
-  (buf: B.buffer U8.t{B.length buf == U32.v l})
-  (crc: U32.t):
-  ST.Stack ((U32.t & (B.buffer U8.t)) & (Ghost.erased (Seq.seq U8.t)))
-  (decreases (U32.v r) - ((U32.v l) % 4))
-  (requires fun h ->
-    B.live h buf /\
-    table_correct 8 h t8 /\
-    B.disjoint t8 buf /\
-    (Ghost.reveal m') == (Ghost.reveal m) + (U32.v r) /\
-    Seq.equal data (prev @| (Seq.slice (B.as_seq h buf) 0 (U32.v r))) /\
-    crc32_matched m' data crc false)
-  (ensures fun h0 res h1 ->
-    let crc' = fst (fst res) in
-    let buf' = snd (fst res) in
-    let data' = Ghost.reveal (snd res) in
-    B.modifies B.loc_none h0 h1 /\
-    (B.length buf') % 4 == 0 /\
-    Seq.length data' == (m + ((U32.v l) % 4)) /\
-    Seq.equal data' (prev @| (Seq.slice (B.as_seq h1 buf) 0 ((U32.v l) % 4))) /\
-    crc32_matched (m + ((U32.v l) % 4)) data' crc' false) =
+inline_for_extraction let rec iteration_1
+  (tg: table_group)
+  (p: crc32_current_state)
+  (d: Ghost.erased crc32_init_state)
+  (base_len: U32.t{U32.v base_len == d.blen})
+  (i: U32.t{U32.v i < d.blen % 4}):
+  ST.Stack (U32.t & (B.buffer U8.t) & (Ghost.erased (Seq.seq U8.t)))
+  (decreases U32.v i - U32.v p.slen % 4)
+  (requires fun h -> do_pre_cond h tg p d (U32.v i) 1)
+  (ensures fun h0 res h1 -> do_post_cond h0 h1 tg p d res (U32.v i) 1 (Some 4)) =
   let open U32 in
-  let (crc', data') = do1 m' data t8 crc (B.index buf r) in
-  if r +^ 1ul <^ l %^ 4ul then begin
-    do1_remain m prev (m + ((v r) + 1)) data' t8 l (r +^ 1ul) buf crc'
-  end else begin
-    let buf' = B.sub buf (r +^ 1ul) (l -^ (r +^ 1ul)) in
-    ((crc', buf'), data')
-  end
+  let (crc', stream', data') = do1 tg p d (v i) in
+  if i +^ 1ul <^ base_len %^ 4ul then begin
+    iteration_1 tg ({
+      clen = p.clen + 1;
+      consumed = data';
+      crc = crc';
+      slen = p.slen -^ 1ul;
+      stream = stream'
+    }) d base_len (i +^ 1ul)
+  end else
+    (crc', stream', data')
 
 inline_for_extraction
-private let dword_seq_to_u32 (a b c d: U8.t): Tot(crc32_data_dword a b c d) =
+let dword_seq_to_u32 (a b c d: U8.t): Tot(crc32_data_dword a b c d) =
   let a' = Cast.uint8_to_uint32 a in
   let b' = Cast.uint8_to_uint32 b in
   let c' = Cast.uint8_to_uint32 c in
@@ -256,7 +297,7 @@ let do4_logxor
     }
 
 #set-options "--z3rlimit 120 --fuel 0 --ifuel 0"
-private let do4_table_lookup
+let do4_table_lookup
   (r: U32.t) (t0: U32.t{
     let open U32 in poly_mod_correct 32 (r &^ 0xFFul) t0
   }) (t1: U32.t{
@@ -311,28 +352,23 @@ private let do4_table_lookup
     (poly_mod_u32 16 r2) +@
     (poly_mod_u32 8 r3)))
 
-#set-options "--z3rlimit 120 --fuel 0 --ifuel 0"
-inline_for_extraction
-private let do4
-  (#m: Ghost.erased nat)
-  (data: Ghost.erased (Seq.seq U8.t){Seq.length data == Ghost.reveal m})
-  (t8 t16 t24 t32: Spec.table_buf)
-  (crc: U32.t)
-  (a b c d: U8.t):
-  ST.Stack (U32.t & (Ghost.erased (Seq.seq U8.t)))
-  (requires fun h ->
-    table_group_correct h t8 t16 t24 t32 /\
-    crc32_matched m data crc false)
-  (ensures fun h0 res h1 ->
-    let crc' = fst res in
-    let data' = Ghost.reveal (snd res) in
-    B.modifies B.loc_none h0 h1 /\
-    data' == data @| (Seq.init 4 (fun i -> match i with | 0 -> a | 1 -> b | 2 -> c | 3 -> d)) /\
-    crc32_matched (m + 4) data' crc' false) =
+inline_for_extraction let do4
+  (tg: table_group)
+  (p: crc32_current_state)
+  (d: Ghost.erased crc32_init_state)
+  (i: Ghost.erased nat):
+  ST.Stack (U32.t & (B.buffer U8.t) & Ghost.erased (Seq.seq U8.t))
+  (requires fun h -> do_pre_cond h tg p d i 4)
+  (ensures fun h0 res h1 -> do_post_cond h0 h1 tg p d res i 4 None) = 
   let open U32 in
+  let a = p.stream.(0ul) in
+  let b = p.stream.(1ul) in
+  let c = p.stream.(2ul) in
+  let d = p.stream.(3ul) in
+  
   let dw = dword_seq_to_u32 a b c d in
   let dw' = Ghost.hide (UInt.to_vec (v dw)) in
-  let r = crc ^^ dw in
+  let r = p.crc ^^ dw in
   let r' = Ghost.hide (UInt.to_vec (v r)) in
   let r0 = r &^ 0xFFul in
   let r1 = (r >>^ 8ul) &^ 0xFFul in
@@ -342,37 +378,149 @@ private let do4
   UInt.logand_le (v (r >>^ 8ul)) 255;
   UInt.logand_le (v (r >>^ 16ul)) 255;
   Math.lemma_div_lt (v r) 32 24;
-  do4_logxor #m data crc a b c d;
+  do4_logxor #p.clen p.consumed p.crc a b c d;
 
+  let (t8, t16, t24, t32) = unfold_table_group tg in
   let t0 = t32.(r0) in let t1 = t24.(r1) in let t2 = t16.(r2) in let t3 = t8.(r3) in
   let crc' = t0 ^^ t1 ^^ t2 ^^ t3 in
   do4_table_lookup r t0 t1 t2 t3 crc';
 
   let seq_32bit = Ghost.hide (crc32_dword_seq a b c d) in
   let buf:
-    Ghost.erased (BV.bv_t (if m > 0 then 32 + 8 * m else 0)) =
-    Ghost.hide (crc32_data_to_bits m data) in
+    Ghost.erased (BV.bv_t (if p.clen > 0 then 32 + 8 * p.clen else 0)) =
+    Ghost.hide (crc32_data_to_bits p.clen p.consumed) in
 
-  assert(poly_mod (zero_vec_l 32 (UInt.to_vec (U32.v r))) == (UInt.to_vec (U32.v crc')));
-  crc32_data_to_bits_append m 4 data seq_32bit;
-  crc32_data_to_bits_32bit m data buf dw;
-  if Ghost.reveal m > 0 then
-    poly_mod_zero_prefix ((zero_vec_r (8 * m) dw') +@ buf) 32
+  crc32_data_to_bits_append p.clen 4 p.consumed seq_32bit;
+  crc32_data_to_bits_32bit p.clen p.consumed buf dw;
+  if Ghost.reveal p.clen > 0 then
+    poly_mod_zero_prefix ((zero_vec_r (8 * p.clen) dw') +@ buf) 32
   else
-    assert(Seq.equal seq_32bit (data @| seq_32bit));
+    assert(Seq.equal seq_32bit (p.consumed @| seq_32bit));
 
-  (crc', Ghost.hide (data @| seq_32bit))
+  (crc', B.sub p.stream 4ul (p.slen -^ 4ul), Ghost.hide (p.consumed @| seq_32bit))
 
-let crc32_impl m data t8 t16 t24 t32 crc buf len =
+inline_for_extraction let rec iteration_4
+  (tg: table_group)
+  (p: crc32_current_state)
+  (d: Ghost.erased crc32_init_state)
+  (base_len: U32.t{U32.v base_len == d.blen})
+  (i: U32.t{U32.v i < d.blen % 32}):
+  ST.Stack (U32.t & (B.buffer U8.t) & (Ghost.erased (Seq.seq U8.t)))
+  (decreases U32.v i - U32.v p.slen % 32)
+  (requires fun h -> do_pre_cond h tg p d (U32.v i) 4)
+  (ensures fun h0 res h1 -> do_post_cond h0 h1 tg p d res (U32.v i) 4 (Some 32)) =
+  let open U32 in
+  let (crc', stream', data') = do4 tg p d (v i) in
+  if i +^ 4ul <^ base_len %^ 32ul then
+    iteration_4 tg ({
+      clen = p.clen + 4;
+      consumed = data';
+      crc = crc';
+      slen = p.slen -^ 4ul;
+      stream = stream';
+    }) d base_len (i +^ 4ul)
+  else
+    (crc', stream', data')
+
+#set-options "--z3rlimit 1024 --fuel 0 --ifuel 0 --z3seed 13"
+inline_for_extraction let do32
+  (tg: table_group)
+  (p: crc32_current_state)
+  (d: Ghost.erased crc32_init_state)
+  (i: Ghost.erased nat):
+  ST.Stack (U32.t & (B.buffer U8.t) & Ghost.erased (Seq.seq U8.t))
+  (requires fun h -> do_pre_cond h tg p d i 32)
+  (ensures fun h0 res h1 -> do_post_cond h0 h1 tg p d res i 32 None) =
+  let open U32 in
+  let mkparam (j: U32.t{
+    4 <= U32.v j /\ U32.v j <= 28 /\ U32.v j % 4 == 0
+  }) c b d: Tot crc32_current_state = {
+    clen = p.clen + (U32.v j);
+    consumed = d;
+    crc = c;
+    slen = p.slen -^ j;
+    stream = b;
+  } in
+  let (c0, b0, d0) = do4 tg p d i in
+  let (c1, b1, d1) = do4 tg (mkparam 4ul c0 b0 d0) d (i + 4) in
+  let (c2, b2, d2) = do4 tg (mkparam 8ul c1 b1 d1) d (i + 8) in
+  let (c3, b3, d3) = do4 tg (mkparam 12ul c2 b2 d2) d (i + 12) in
+  let (c4, b4, d4) = do4 tg (mkparam 16ul c3 b3 d3) d (i + 16) in
+  let (c5, b5, d5) = do4 tg (mkparam 20ul c4 b4 d4) d (i + 20) in
+  let (c6, b6, d6) = do4 tg (mkparam 24ul c5 b5 d5) d (i + 24) in
+  let (c7, b7, d7) = do4 tg (mkparam 28ul c6 b6 d6) d (i + 28) in
+  (c7, b7, d7)
+
+inline_for_extraction let rec iteration_32
+  (tg: table_group)
+  (p: crc32_current_state)
+  (d: Ghost.erased crc32_init_state)
+  (base_len: U32.t{U32.v base_len == d.blen})
+  (i: Ghost.erased nat{i + 32 <= d.blen}):
+  ST.Stack (U32.t & (B.buffer U8.t) & (Ghost.erased (Seq.seq U8.t)))
+  (decreases d.blen - i)
+  (requires fun h -> do_pre_cond h tg p d i 32)
+  (ensures fun h0 res h1 -> do_post_cond h0 h1 tg p d res i 32 (Some 0)) =
+  let open U32 in
+  let (crc', buf', data') = do32 tg p d i in
+  if p.slen -^ 32ul >=^ 32ul then
+    iteration_32 tg ({
+      clen = p.clen + 32;
+      consumed = data';
+      crc = crc';
+      slen = p.slen -^ 32ul;
+      stream = buf';
+    }) d base_len (i + 32)
+  else
+    (crc', buf', data')
+
+type it_tuple = (U32.t & (B.buffer U8.t) & U32.t & Ghost.erased (Seq.seq U8.t))
+
+let crc32_impl tg crc len buf d =
   let open U32 in
   ST.push_frame ();
-  let crc' = crc ^^ 0xfffffffful in
-  crc32_matched_xor_inv_1 m data crc;
-  let ((c0, buf'), data') = if len %^ 4ul >^ 0ul then
-    do1_remain m data m data t8 len 0ul buf crc'
-  else
-    ((crc', buf), data)
+  let crc' = crc ^^ 0xFFFFFFFFul in
+  crc32_matched_xor_inv_1 d.dlen d.data crc;
+  
+  let (c0, b0, l0, d0): it_tuple = if len %^ 4ul >^ 0ul then begin
+    let (c', b', d') = iteration_1 tg ({
+      clen = d.dlen;
+      consumed = d.data; 
+      crc = crc';
+      slen = len;
+      stream = buf;
+    }) d len 0ul
+    in
+    (c', b', len -^ (len %^ 4ul), d')
+  end else
+    (crc', buf, len, Ghost.hide d.data)
   in
-  admit();
+  let (c1, b1, l1, d1): it_tuple = if l0 %^ 32ul >^ 0ul then
+    let (c', b', d') = iteration_4 tg ({
+      clen = d.dlen + v (len -^ l0);
+      consumed = d0;
+      crc = c0;
+      slen = l0;
+      stream = b0;
+    }) d len (len -^ l0)
+    in
+    (c', b', l0 -^ (l0 %^ 32ul), d')
+  else
+    (c0, b0, l0, d0)
+  in
+  let (c2, d2): (U32.t & Ghost.erased (Seq.seq U8.t))  = if l1 >^ 0ul then
+    let (c', _, d') = iteration_32 tg ({
+      clen = d.dlen + v (len -^ l1);
+      consumed = d1;
+      crc = c1;
+      slen = l1;
+      stream = b1;
+    }) d len (U32.v (len -^ l1))
+    in
+    (c', d')
+  else
+    (c1, d1)
+  in
   ST.pop_frame ();
-  c0
+  crc32_matched_xor_inv_2 (d.dlen + v len) d2 c2;
+  c2 ^^ 0xFFFFFFFFul
