code/Yazi.CRC32.fsti
@@ -1,40 +1,95 @@
 module Yazi.CRC32
 
 module B = LowStar.Buffer
-module BV = FStar.BitVector
 module Ghost = FStar.Ghost
 module HS = FStar.HyperStack
-module M = LowStar.Modifies
 module U32 = FStar.UInt32
 module U8 = FStar.UInt8
 module Seq = FStar.Seq
 module Spec = Spec.CRC32
 module ST = FStar.HyperStack.ST
 
-private unfold let table_group_correct h t8 t16 t24 t32 =
+private type table_group = t: B.buffer U32.t{B.length t == 1024}
+
+private unfold let unfold_table_group_ghost (t: table_group):
+  GTot (Spec.table_buf & Spec.table_buf & Spec.table_buf & Spec.table_buf) =
+  let t8 = B.gsub t 0ul 256ul in
+  let t16 = B.gsub t 256ul 256ul in
+  let t24 = B.gsub t 512ul 256ul in
+  let t32 = B.gsub t 768ul 256ul in
+  (t8, t16, t24, t32)
+
+private unfold let table_group_correct_pre (h: HS.mem) (tg:table_group) =
+  B.live h tg /\
+  (let (t8, t16, t24, t32) = unfold_table_group_ghost tg in
   Spec.table_correct 8 h t8 /\
   Spec.table_correct 16 h t16 /\
   Spec.table_correct 24 h t24 /\
   Spec.table_correct 32 h t32 /\
   B.disjoint t8 t16 /\ B.disjoint t8 t24 /\ B.disjoint t8 t32 /\
-  B.disjoint t16 t24 /\ B.disjoint t16 t32 /\ B.disjoint t24 t32
+  B.disjoint t16 t24 /\ B.disjoint t16 t32 /\ B.disjoint t24 t32)
 
+private unfold let table_group_correct_post (h: HS.mem) (t8 t16 t24 t32: Spec.table_buf) =
+  Spec.table_correct 8 h t8 /\
+  Spec.table_correct 16 h t16 /\
+  Spec.table_correct 24 h t24 /\
+  Spec.table_correct 32 h t32 /\
+  B.disjoint t8 t16 /\ B.disjoint t8 t24 /\ B.disjoint t8 t32 /\
+  B.disjoint t16 t24 /\ B.disjoint t16 t32 /\ B.disjoint t24 t32 /\
+  B.live h t8 /\ B.live h t16 /\ B.live h t24 /\ B.live h t32
+
+private let unfold_table_group (tg: table_group):
+  ST.Stack (Spec.table_buf & Spec.table_buf & Spec.table_buf & Spec.table_buf)
+  (requires fun h -> table_group_correct_pre h tg)
+  (ensures fun h0 res h1 ->
+    B.modifies B.loc_none h0 h1 /\
+    (let (t8, t16, t24, t32) = res in
+    B.live h1 t8 /\ B.live h1 t16 /\ B.live h1 t24 /\ B.live h1 t32 /\
+    table_group_correct_post h1 t8 t16 t24 t32)) =
+  let t8 = B.sub tg 0ul 256ul in
+  let t16 = B.sub tg 256ul 256ul in
+  let t24 = B.sub tg 512ul 256ul in
+  let t32 = B.sub tg 768ul 256ul in
+  (t8, t16, t24, t32)
+
+private noeq type crc32_current_state = {
+  clen: Ghost.erased nat;
+  consumed: Ghost.erased (Seq.seq U8.t);
+  crc: U32.t;
+  slen: U32.t;
+  stream: B.buffer U8.t;
+}
+
+private noeq type crc32_init_state = {
+  dlen: nat;
+  blen: nat;
+  base: B.buffer U8.t;
+  data: Seq.seq U8.t;
+}
+
+private let crc32_pre_cond
+  (h: HS.mem)
+  (crc len: U32.t)
+  (buf: B.buffer U8.t)
+  (d: crc32_init_state) =
+  let len' = U32.v len in
+  d.base == buf /\ B.live h buf /\
+  B.length buf == len' /\ B.length d.base == d.blen /\ Seq.length d.data == d.dlen /\
+  Spec.crc32_matched d.dlen d.data crc true
+
+[@ (CPrologue
+  "unsigned long crc32(unsigned int crc, const unsigned char *buf, unsigned int len);")]
 val crc32_impl:
-    n: Ghost.erased nat
-  -> data: Ghost.erased (Seq.seq U8.t){Seq.length data == Ghost.reveal n}
-  -> t8: Spec.table_buf
-  -> t16: Spec.table_buf
-  -> t24: Spec.table_buf
-  -> t32: Spec.table_buf
+    tg: table_group
   -> crc: U32.t
+  -> len: U32.t
   -> buf: B.buffer U8.t
-  -> len: U32.t{B.length buf == U32.v len}
+  -> d: Ghost.erased crc32_init_state
   -> ST.Stack U32.t
   (requires fun h ->
-    B.live h buf /\
-    B.disjoint buf t8 /\ B.disjoint buf t16 /\ B.disjoint buf t24 /\ B.disjoint buf t32 /\
-    table_group_correct h t8 t16 t24 t32 /\
-    Spec.crc32_matched n data crc true)
+    crc32_pre_cond h crc len buf d /\
+    B.disjoint buf tg /\
+    table_group_correct_pre h tg)
   (ensures fun h0 res h1 ->
-    M.modifies B.loc_none h0 h1 /\
-    Spec.crc32_matched (n + U32.v len) (Seq.append data (B.as_seq h1 buf)) crc true)
+    B.(modifies loc_none h0 h1) /\
+    Spec.crc32_matched (d.dlen + U32.v len) (Seq.append d.data (B.as_seq h1 buf)) res true)
